split lifting.v into three files

fairis/heap_lang/lifting.v
@@ -1,219 +1,9 @@
-From stdpp Require Import fin_maps.
 From iris.proofmode Require Import tactics.
-From iris.algebra Require Import auth gmap gset excl.
-From iris.base_logic Require Export gen_heap.
-From trillium.prelude Require Import classical_instances.
-From trillium.program_logic Require Export weakestpre adequacy.
-From trillium.fairness Require Export fairness fair_termination fuel fuel_termination action_model.
-From trillium.fairness.lm_rules Require Import lm_rules.
 From trillium.program_logic Require Import ectx_lifting.
-From trillium.fairness.heap_lang Require Export lang.
-From trillium.fairness.heap_lang Require Import tactics notation.
-Set Default Proof Using "Type".
-
-(* Canonical Structure ModelO (M : FairModel) := leibnizO M. *)
-(* Canonical Structure RoleO (M : FairModel) := leibnizO (M.(fmrole)). *)
-
-(* Class heapGpreS Σ `(LM: LiveModel heap_lang M) := HeapPreG { *)
-Class heapGpreS Σ (AM1 AM2: ActionModel) := HeapPreG {
-  heapGpreS_inv :> invGpreS Σ;
-  heapGpreS_gen_heap :> gen_heapGpreS loc val Σ;
-  heapGpreS_fairness :> fairnessGpreS AM1 AM2 Σ;
-}.
-
-(* Class heapGS Σ `(LM:LiveModel heap_lang M) := HeapG { *)
-Class heapGS Σ (AM1 AM2: ActionModel) := HeapG { 
-  heap_inG :> heapGpreS Σ AM1 AM2;
-  heap_invGS : invGS_gen HasNoLc Σ;
-  heap_gen_heapGS :> gen_heapGS loc val Σ;
-  heap_fairnessGS :> fairnessGS AM1 AM2 Σ;
-}.
-
-Definition heapΣ (AM1 AM2: ActionModel) : gFunctors :=
-  #[ invΣ; gen_heapΣ loc val; fairnessΣ heap_lang AM1 AM2 ].
-
-Global Instance subG_heapPreG {Σ} {AM1 AM2: ActionModel} :
-  subG (heapΣ AM1 AM2) Σ → heapGpreS Σ AM1 AM2.
-Proof. solve_inG. Qed.
-
-#[global] Instance heapG_irisG {AM1 AM2: ActionModel} 
-  (PM := ProdAM AM1 AM2)
-  {PMS: AM_strong_lr PM}
-  (M := AM2FM PM PMS)
-  {LM: LiveModel heap_lang M}
- `{!heapGS Σ AM1 AM2} : irisG heap_lang LM Σ := {
-    iris_invGS := heap_invGS;
-    state_interp extr auxtr :=
-      (⌜valid_state_evolution_fairness extr auxtr⌝ ∗
-       gen_heap_interp (trace_last extr).2.(heap) ∗
-       model_state_interp (trace_last extr).1 (trace_last auxtr))%I ;
-    fork_post tid := λ _, (tid ↦M ∅)%I;
-}.
-
-(** Override the notations so that scopes and coercions work out *)
-Notation "l ↦{ q } v" := (pointsto (L:=loc) (V:=val) l (DfracOwn q) v%V)
-  (at level 20, q at level 50, format "l  ↦{ q }  v") : bi_scope.
-Notation "l ↦ v" :=
-  (pointsto (L:=loc) (V:=val) l (DfracOwn 1) v%V) (at level 20) : bi_scope.
-Notation "l ↦{ q } -" := (∃ v, l ↦{q} v)%I
-  (at level 20, q at level 50, format "l  ↦{ q }  -") : bi_scope.
-Notation "l ↦ -" := (l ↦{1} -)%I (at level 20) : bi_scope.
-
-(** The tactic [inv_head_step] performs inversion on hypotheses of the shape
-[head_step]. The tactic will discharge head-reductions starting from values, and
-simplifies hypothesis related to conversions from and to values, and finite map
-operations. This tactic is slightly ad-hoc and tuned for proving our lifting
-lemmas. *)
-Ltac inv_head_step :=
-  repeat match goal with
-  | _ => progress simplify_map_eq/= (* simplify memory stuff *)
-  | H : to_val _ = Some _ |- _ => apply of_to_val in H
-  | H : head_step ?e _ _ _ _ |- _ =>
-     try (is_var e; fail 1); (* inversion yields many goals if [e] is a variable
-     and can thus better be avoided. *)
-     inversion H; subst; clear H
-  end.
-
-Local Hint Extern 0 (head_reducible _ _) => eexists _, _, _; simpl : core.
-Local Hint Extern 1 (head_step _ _ _ _ _) => econstructor : core.
-Local Hint Extern 0 (head_step (CmpXchg _ _ _) _ _ _ _) => eapply CmpXchgS : core.
-Local Hint Extern 0 (head_step (AllocN _ _) _ _ _ _) => apply alloc_fresh : core.
-Local Hint Resolve to_of_val : core.
-
-#[global] Instance into_val_val v : IntoVal (Val v) v.
-Proof. done. Qed.
-#[global] Instance as_val_val v : AsVal (Val v).
-Proof. by eexists. Qed.
-
-Local Ltac solve_atomic :=
-  apply strongly_atomic_atomic, ectx_language_atomic;
-    [inversion 1; naive_solver
-    |apply ectxi_language_sub_redexes_are_values; intros [] **; naive_solver].
-
-#[global] Instance rec_atomic s f x e : Atomic s (Rec f x e).
-Proof. solve_atomic. Qed.
-#[global] Instance pair_atomic s v1 v2 : Atomic s (Pair (Val v1) (Val v2)).
-Proof. solve_atomic. Qed.
-#[global] Instance injl_atomic s v : Atomic s (InjL (Val v)).
-Proof. solve_atomic. Qed.
-#[global] Instance injr_atomic s v : Atomic s (InjR (Val v)).
-Proof. solve_atomic. Qed.
-(** The instance below is a more general version of [Skip] *)
-#[global] Instance beta_atomic s f x v1 v2 : Atomic s (App (RecV f x (Val v1)) (Val v2)).
-Proof. destruct f, x; solve_atomic. Qed.
-#[global] Instance unop_atomic s op v : Atomic s (UnOp op (Val v)).
-Proof. solve_atomic. Qed.
-#[global] Instance binop_atomic s op v1 v2 : Atomic s (BinOp op (Val v1) (Val v2)).
-Proof. solve_atomic. Qed.
-#[global] Instance if_true_atomic s v1 e2 : Atomic s (If (Val $ LitV $ LitBool true) (Val v1) e2).
-Proof. solve_atomic. Qed.
-#[global] Instance if_false_atomic s e1 v2 : Atomic s (If (Val $ LitV $ LitBool false) e1 (Val v2)).
-Proof. solve_atomic. Qed.
-#[global] Instance fst_atomic s v : Atomic s (Fst (Val v)).
-Proof. solve_atomic. Qed.
-#[global] Instance snd_atomic s v : Atomic s (Snd (Val v)).
-Proof. solve_atomic. Qed.
-
-#[global] Instance fork_atomic s e : Atomic s (Fork e).
-Proof. solve_atomic. Qed.
-
-#[global] Instance allocN_atomic s v w : Atomic s (AllocN (Val v) (Val w)).
-Proof. solve_atomic. Qed.
-#[global] Instance alloc_atomic s v : Atomic s (Alloc (Val v)).
-Proof. solve_atomic. Qed.
-#[global] Instance load_atomic s v : Atomic s (Load (Val v)).
-Proof. solve_atomic. Qed.
-#[global] Instance store_atomic s v1 v2 : Atomic s (Store (Val v1) (Val v2)).
-Proof. solve_atomic. Qed.
-#[global] Instance cmpxchg_atomic s v0 v1 v2 : Atomic s (CmpXchg (Val v0) (Val v1) (Val v2)).
-Proof. solve_atomic. Qed.
-#[global] Instance faa_atomic s v1 v2 : Atomic s (FAA (Val v1) (Val v2)).
-Proof. solve_atomic. Qed.
-
-Local Ltac solve_exec_safe := intros; subst; do 3 eexists; econstructor; eauto.
-Local Ltac solve_exec_puredet := simpl; intros; by inv_head_step.
-Local Ltac solve_pure_exec :=
-  subst; intros ?; apply nsteps_once, pure_head_step_pure_step;
-    constructor; [solve_exec_safe | solve_exec_puredet].
-
-(** The behavior of the various [wp_] tactics with regard to lambda differs in
-the following way:
-
-- [wp_pures] does *not* reduce lambdas/recs that are hidden behind a definition.
-- [wp_rec] and [wp_lam] reduce lambdas/recs that are hidden behind a definition.
-
-To realize this behavior, we define the class [AsRecV v f x erec], which takes a
-value [v] as its input, and turns it into a [RecV f x erec] via the instance
-[AsRecV_recv : AsRecV (RecV f x e) f x e]. We register this instance via
-[Hint Extern] so that it is only used if [v] is syntactically a lambda/rec, and
-not if [v] contains a lambda/rec that is hidden behind a definition.
-
-To make sure that [wp_rec] and [wp_lam] do reduce lambdas/recs that are hidden
-behind a definition, we activate [AsRecV_recv] by hand in these tactics. *)
-Class AsRecV (v : val) (f x : binder) (erec : expr) :=
-  as_recv : v = RecV f x erec.
-#[global] Hint Mode AsRecV ! - - - : typeclass_instances.
-Definition AsRecV_recv f x e : AsRecV (RecV f x e) f x e := eq_refl.
-#[global] Hint Extern 0 (AsRecV (RecV _ _ _) _ _ _) =>
-  apply AsRecV_recv : typeclass_instances.
-
-#[global] Instance pure_recc f x (erec : expr) :
-  PureExec True 1 (Rec f x erec) (Val $ RecV f x erec).
-Proof. solve_pure_exec. Qed.
-#[global] Instance pure_pairc (v1 v2 : val) :
-  PureExec True 1 (Pair (Val v1) (Val v2)) (Val $ PairV v1 v2).
-Proof. solve_pure_exec. Qed.
-#[global] Instance pure_injlc (v : val) :
-  PureExec True 1 (InjL $ Val v) (Val $ InjLV v).
-Proof. solve_pure_exec. Qed.
-#[global] Instance pure_injrc (v : val) :
-  PureExec True 1 (InjR $ Val v) (Val $ InjRV v).
-Proof. solve_pure_exec. Qed.
-
-#[global] Instance pure_beta f x (erec : expr) (v1 v2 : val) `{!AsRecV v1 f x erec} :
-  PureExec True 1 (App (Val v1) (Val v2)) (subst' x v2 (subst' f v1 erec)).
-Proof. unfold AsRecV in *. solve_pure_exec. Qed.
-
-#[global] Instance pure_unop op v v' :
-  PureExec (un_op_eval op v = Some v') 1 (UnOp op (Val v)) (Val v').
-Proof. solve_pure_exec. Qed.
-
-#[global] Instance pure_binop op v1 v2 v' :
-  PureExec (bin_op_eval op v1 v2 = Some v') 1 (BinOp op (Val v1) (Val v2)) (Val v') | 10.
-Proof. solve_pure_exec. Qed.
-(* Higher-priority instance for [EqOp]. *)
-#[global] Instance pure_eqop v1 v2 :
-  PureExec (vals_compare_safe v1 v2) 1
-    (BinOp EqOp (Val v1) (Val v2))
-    (Val $ LitV $ LitBool $ bool_decide (v1 = v2)) | 1.
-Proof.
-  intros Hcompare.
-  cut (bin_op_eval EqOp v1 v2 = Some $ LitV $ LitBool $ bool_decide (v1 = v2)).
-  { intros. revert Hcompare. solve_pure_exec. }
-  rewrite /bin_op_eval /= decide_True //.
-Qed.
-
-#[global] Instance pure_if_true e1 e2 : PureExec True 1 (If (Val $ LitV $ LitBool true) e1 e2) e1.
-Proof. solve_pure_exec. Qed.
-
-#[global] Instance pure_if_false e1 e2 : PureExec True 1 (If (Val $ LitV  $ LitBool false) e1 e2) e2.
-Proof. solve_pure_exec. Qed.
-
-#[global] Instance pure_fst v1 v2 :
-  PureExec True 1 (Fst (Val $ PairV v1 v2)) (Val v1).
-Proof. solve_pure_exec. Qed.
-
-#[global] Instance pure_snd v1 v2 :
-  PureExec True 1 (Snd (Val $ PairV v1 v2)) (Val v2).
-Proof. solve_pure_exec. Qed.
-
-#[global] Instance pure_case_inl v e1 e2 :
-  PureExec True 1 (Case (Val $ InjLV v) e1 e2) (App e1 (Val v)).
-Proof. solve_pure_exec. Qed.
-
-#[global] Instance pure_case_inr v e1 e2 :
-  PureExec True 1 (Case (Val $ InjRV v) e1 e2) (App e2 (Val v)).
-Proof. solve_pure_exec. Qed.
+From trillium.fairness.heap_lang Require Import iris_inst.
+From trillium.fairness Require Import action_model fuel.
+From trillium.fairness.lm_rules Require Import lm_rules.
+From trillium.fairness.heap_lang Require Export lang tactics notation.
 
 Section lifting.
 (* Context `{LM:LiveModel heap_lang M}. *)
@@ -241,159 +31,11 @@ Implicit Types v : val.
 Implicit Types l : loc.
 Implicit Types tid : nat.
 
-Definition sswp (s : stuckness) E e1 (Φ : expr → iProp Σ) : iProp Σ :=
-  match to_val e1 with
-  | Some v => |={E}=> (Φ (of_val v))
-  | None => ∀ σ1,
-      gen_heap_interp σ1.(heap) ={E,∅}=∗
-       ⌜if s is NotStuck then reducible e1 σ1 else True⌝ ∗
-       ∀ e2 σ2 efs,
-         ⌜prim_step e1 σ1 e2 σ2 efs⌝ ={∅}▷=∗ |={∅,E}=>
-         gen_heap_interp σ2.(heap) ∗ Φ e2 ∗ ⌜efs = []⌝
-  end%I.
 
-Lemma sswp_wand s e E (Φ Ψ : expr → iProp Σ) :
-  (∀ e, Φ e -∗ Ψ e) -∗ sswp s E e Φ -∗ sswp s E e Ψ.
-Proof.
-  rewrite /sswp. iIntros "HΦΨ HΦ".
-  destruct (to_val e); [by iApply "HΦΨ"|].
-  iIntros (?) "H". iMod ("HΦ" with "H") as "[%Hs HΦ]".
-  iModIntro. iSplit; [done|]. iIntros (????).
-  iDestruct ("HΦ" with "[//]") as "HΦ".
-  iMod "HΦ". iIntros "!>!>". iMod "HΦ". iIntros "!>". iMod "HΦ" as "(?&?&?)".
-  iIntros "!>". iFrame. by iApply "HΦΨ".
-Qed.
-
-  Definition HL_LM_trace_interp' (extr: execution_trace heap_lang)
-    (lmtr: auxiliary_trace LM) (τ: locale heap_lang): iProp Σ :=
-    match extr with
-    | {tr[ _ ]} => False
-    | extr' :tr[oζ]: c' =>
-        let c := trace_last extr' in
-        let δ := trace_last lmtr in
-        gen_heap_interp c'.2.(heap) ∗
-        model_state_interp c.1 δ ∗
-        ⌜ tids_smaller c.1 δ ⌝ ∗
-        ⌜ oζ = Some τ ⌝ ∗
-        ⌜ locale_step c (Some τ) c' ⌝
-    end.
-
-    Definition MU E ζ (P : iProp Σ) : iProp Σ :=
-    ∀ extr atr,
-      HL_LM_trace_interp' extr atr ζ ={E}=∗
-      ∃ δ2 ℓ, state_interp extr (trace_extend atr ℓ δ2) ∗ P.
-
-    (* TODO: unify with existing locales_of_list_from_locale_from, 
-       remove restriction for Λ *)
-    Lemma locales_of_list_from_locale_from' {Λ: language} `{EqDecision (locale Λ)}
-      tp0 tp1 ζ:
-      ζ ∈ locales_of_list_from tp0 tp1 (Λ := Λ) ->
-      is_Some (from_locale_from tp0 tp1 ζ).
-    Proof.
-      clear -tp0 tp1 ζ.
-      revert tp0; induction tp1 as [|e1 tp1 IH]; intros tp0.
-      { simpl. intros H. inversion H. }
-      simpl.
-      rewrite /locales_of_list_from /=. intros.
-      destruct (decide (language.locale_of tp0 e1 = ζ)); simplify_eq; first set_solver.
-      apply elem_of_cons in H as [?| ?]; [done| ].
-      set_solver.
-    Qed.
-
-    (* TODO: have similar proof in other repo *)
-    Lemma MSI_tids_smaller (σ: list expr) δ:
-      ⊢ model_state_interp σ δ -∗ ⌜tids_smaller σ δ⌝.
-    Proof. 
-      rewrite /model_state_interp.
-      iIntros "(%fm & %LE & %DEAD & %TP & X)".
-      iPureIntro. red. intros.
-      apply locales_of_list_from_locale_from'.
-      destruct (decide (ζ ∈ locales_of_list σ)); [done| ].
-      red in TP. specialize (TP _ n).
-      red in LE. apply proj2 in LE. rewrite -LE in H.
-      by apply not_elem_of_dom in TP. 
-    Qed. 
 
     (* TODO: move *)
     Lemma locale_fill' e K t1: locale_of t1 (fill K e) = locale_of t1 e.
     Proof. done. Qed.
-
-
-  Lemma sswp_MU_wp_fupd s E E' ζ e Φ
-    (NVAL: language.to_val e = None)
-    :
-    let sswp_post := λ e', (MU E' ζ ((|={E',E}=> WP e' @ s; ζ; E {{ Φ }})))%I in
-      (|={E,E'}=> sswp s E' e sswp_post)%I -∗
-      WP e @ s; ζ; E {{ Φ }}.
-  Proof.
-    simpl. rewrite wp_unfold /wp_pre.
-    iIntros "Hsswp". rewrite NVAL. 
-    iIntros (extr atr K tp1 tp2 σ1 Hvalid Hζ Hextr) "Hσ".
-    iMod "Hsswp" as "foo".
-    rewrite /sswp. rewrite NVAL.
-    iSimpl in "Hσ". iDestruct "Hσ" as "(%EV & HEAP & MSI)".
-    iSpecialize ("foo" with "HEAP").
-    iMod "foo" as (Hs) "Hsswp".
-    red in Hextr. rewrite Hextr. 
-    iModIntro. iSplit.
-    { iPureIntro. by rewrite Hextr in Hs. }
-    iIntros (e2 σ2 efs Hstep).
-    iDestruct ("Hsswp" with "[//]") as "Hsswp".
-    iApply (step_fupdN_le 1); [| done| ].
-    { pose proof (trace_length_at_least extr). lia. }
-    simpl.
-    iApply (step_fupd_wand with "Hsswp").
-    iIntros ">(Hσ & HMU & ->)".
-    rewrite /MU. iSpecialize ("HMU" $! (_ :tr[Some ζ]: _)  with "[MSI Hσ]").
-    { rewrite /HL_LM_trace_interp'.
-      iPoseProof (MSI_tids_smaller with "MSI") as "%TS".
-      remember (trace_last extr) as xx. destruct xx as [tp h].
-      inversion Hextr as [[TP H]]. 
-      rewrite -TP in TS. 
-      iApply bi.sep_assoc. iSplitL.
-      2: { iPureIntro. repeat split; eauto.
-           { replace tp with (tp, h).1 in TS by done.
-             rewrite Heqxx in TS. apply TS. }
-           simpl in Hζ. 
-           rewrite -Hζ. simpl.
-           (* rewrite locale_fill'.  *)
-           eapply locale_step_atomic.
-           3: { eapply @fill_step. apply Hstep. } 
-           { rewrite -Heqxx Hextr. simpl. reflexivity. }
-           reflexivity. }
-      rewrite -Heqxx TP. simpl. iFrame. }
-    iMod ("HMU") as (??) "[Hσ Hwp]". iMod "Hwp". iModIntro.
-    iExists _, _. rewrite right_id_L. by iFrame.
-  Qed.
-
-  Lemma MU_wand E ζ (P Q : iProp Σ) :
-    (P -∗ Q) -∗ MU E ζ P -∗ MU E ζ Q.
-  Proof.
-    rewrite /MU. iIntros "HPQ HMU".
-    iIntros (extr atr) "Hσ".
-    iMod ("HMU" with "Hσ") as (??) "[Hσ HP]". iModIntro.
-    iExists _, _. iFrame. by iApply "HPQ".
-  Qed.
-
-  Lemma MU_mask_weaken E1 E2 ζ (P: iProp Σ)
-    (SUB: E1 ⊆ E2):
-    MU E1 ζ P -∗ MU E2 ζ P.
-  Proof.
-    rewrite /MU. iIntros "MU".
-    iIntros "**".
-    iApply fupd_mask_mono; eauto.
-    by iApply "MU". 
-  Qed.
-
-  Lemma sswp_MU_wp s E ζ e (Φ : val → iProp Σ)
-    (NVAL: language.to_val e = None):
-    sswp s E e (λ e', MU E ζ (WP e' @ s; ζ;  E {{ Φ }})) -∗
-      WP e @ s; ζ; E {{ Φ }}.
-  Proof.
-    iIntros "Hsswp". iApply sswp_MU_wp_fupd; auto. iModIntro.
-    iApply (sswp_wand with "[] Hsswp").
-    iIntros (?) "HMU". iApply (MU_wand with "[] HMU"). by iIntros "$ !>".
-  Qed.
 
 
 Lemma has_fuels_decr E tid fs :
@@ -435,7 +77,7 @@ Lemma model_step_MU tid E s1 s2 ρ f1 fs a
   frag_model_is s1 -∗
   tid ↦M ({[inl ρ := f1]} ∪ (S <$> fs)) -∗
   MU E tid (frag_model_is s2 ∗
-           tid ↦M ({[inl ρ := lm_flm LM]} ∪ fs)).
+           tid ↦M ({[inl ρ := lm_flm LM]} ∪ fs)) (LM := LM).
 Proof using LR1 LR2 INDEP.
   iIntros "Hst Hfuel1".
   rewrite /MU /HL_LM_trace_interp'. iIntros (extr lmtr) "X".
@@ -459,7 +101,7 @@ Lemma wp_step_model s tid ρ (f1 : nat) fs s1 s2 a E e Φ :
   ▷ tid ↦M ({[inl ρ:=f1]} ∪ fmap S fs) -∗
   sswp s E e (λ e', frag_model_is s2 -∗
                     tid ↦M ({[inl ρ:=(LM.(lm_flm))]} ∪ fs) -∗
-                    WP e' @ s; tid; E {{ Φ }} ) -∗
+                    WP e' @ s; tid; E {{ Φ }} ) (LM := LM) -∗
   WP e @ s; tid; E {{ Φ }}.
 Proof using LR1 LR2 INDEP.
   iIntros (Hval Htrans Hlive Hdom) ">Hst >Hfuel1 Hwp".
@@ -473,7 +115,6 @@ Proof using LR1 LR2 INDEP.
 Qed. 
 
 
-
 Lemma wp_step_model_singlerole s tid ρ (f1 : nat) s1 s2 a E e Φ :
   TCEq (to_val e) None →
   (* fmtrans M s1 (Some ρ) s2 → *)
@@ -483,7 +124,7 @@ Lemma wp_step_model_singlerole s tid ρ (f1 : nat) s1 s2 a E e Φ :
   ▷ frag_model_is s1 -∗ ▷ tid ↦M {[inl ρ := f1]} -∗
   sswp s E e (λ e', frag_model_is s2 -∗
                     tid ↦M {[inl ρ := (LM.(lm_flm))]} -∗
-                    WP e' @ s; tid; E {{ Φ }} ) -∗
+                    WP e' @ s; tid; E {{ Φ }} ) (LM := LM) -∗
   WP e @ s; tid; E {{ Φ }}.
 Proof using LR1 LR2 INDEP.
   iIntros (Hval Htrans Hlive) ">Hst >Hfuel1 Hwp".
@@ -496,7 +137,7 @@ Qed.
 
 Lemma wp_step_fuel s tid E e fs Φ :
   fs ≠ ∅ → ▷ tid ↦M++ fs -∗
-  sswp s E e (λ e', tid ↦M fs -∗ WP e' @ s; tid; E {{ Φ }} ) -∗
+  sswp s E e (λ e', tid ↦M fs -∗ WP e' @ s; tid; E {{ Φ }} ) (LM := LM)-∗
   WP e @ s; tid; E {{ Φ }}.
 Proof using INDEP.
   iIntros (?) ">HfuelS Hwp". rewrite wp_unfold /wp_pre /sswp /=.
@@ -557,218 +198,14 @@ Proof.
     split; first by list_simplifier.
     apply heap_lang_locales_equiv_length. simpl.
     rewrite !app_length //=. }
-  iModIntro. iSplit. iPureIntro; first by eauto. iNext.
+  iModIntro. iSplit.
+  { iPureIntro. by eauto. }
   iIntros (e2 σ2 efs Hstep).
   have [-> [-> ->]] : σ2 = σ1 ∧ efs = [e] ∧ e2 = Val $ LitV LitUnit by inv_head_step.
+  iNext. 
   iMod ("HΦ" with "Hfuels1") as "HΦ". iModIntro. iExists δ2, (Silent_step tid).
   iFrame. rewrite Hexend /=. iFrame "Hsi". iSplit; [by iPureIntro|].
   iSplit; [|done]. iApply "He". by list_simplifier.
-Qed.
-
-Lemma sswp_pure_step s E e1 e2 (Φ : Prop) Ψ :
-  PureExec Φ 1 e1 e2 → Φ → ▷ Ψ e2 -∗ sswp s E e1 Ψ%I.
-Proof.
-  clear INDEP. 
-  iIntros (Hpe HΦ) "HΨ".
-  assert (pure_step e1 e2) as Hps.
-  { specialize (Hpe HΦ). by apply nsteps_once_inv in Hpe. }
-  rewrite /sswp /=.
-  assert (to_val e1 = None) as ->.
-  { destruct Hps as [Hred _]. specialize (Hred (Build_state ∅ ∅)).
-    by eapply reducible_not_val. }
-  iIntros (σ) "Hσ".
-  iMod fupd_mask_subseteq as "Hclose"; last iModIntro; [by set_solver|].
-  iSplit.
-  { destruct s; [|done]. by destruct Hps as [Hred _]. }
-  iIntros (e2' σ2 efs Hstep) "!>!>!>".
-  iMod "Hclose". iModIntro. destruct Hps as [_ Hstep'].
-  apply Hstep' in Hstep as [-> [-> ->]]. by iFrame.
-Qed.
-
-(** Heap *)
-(** The usable rules for [allocN] stated in terms of the [array] proposition
-are derived in te file [array]. *)
-Lemma heap_array_to_seq_meta l vs (n : nat) :
-  length vs = n →
-  ([∗ map] l' ↦ _ ∈ heap_array l vs, meta_token l' ⊤) -∗
-  [∗ list] i ∈ seq 0 n, meta_token (l +ₗ (i : nat)) ⊤.
-Proof.
-  iIntros (<-) "Hvs". iInduction vs as [|v vs] "IH" forall (l)=> //=.
-  rewrite big_opM_union; last first.
-  { apply map_disjoint_spec=> l' v1 v2 /lookup_singleton_Some [-> _].
-    intros (j&?&Hjl&_)%heap_array_lookup.
-    rewrite loc_add_assoc -{1}[l']loc_add_0 in Hjl. simplify_eq; lia. }
-  rewrite loc_add_0 -fmap_S_seq big_sepL_fmap.
-  setoid_rewrite Nat2Z.inj_succ. setoid_rewrite <-Z.add_1_l.
-  setoid_rewrite <-loc_add_assoc.
-  rewrite big_opM_singleton; iDestruct "Hvs" as "[$ Hvs]". by iApply "IH".
-Qed.
-
-Lemma heap_array_to_seq_mapsto l v (n : nat) :
-  ([∗ map] l' ↦ v ∈ heap_array l (replicate n v), l' ↦ v) -∗
-  [∗ list] i ∈ seq 0 n, (l +ₗ (i : nat)) ↦ v.
-Proof.
-  iIntros "Hvs". iInduction n as [|n] "IH" forall (l); simpl.
-  { done. }
-  rewrite big_opM_union; last first.
-  { apply map_disjoint_spec=> l' v1 v2 /lookup_singleton_Some [-> _].
-    intros (j&?&Hjl&_)%heap_array_lookup.
-    rewrite loc_add_assoc -{1}[l']loc_add_0 in Hjl. simplify_eq; lia. }
-  rewrite loc_add_0 -fmap_S_seq big_sepL_fmap.
-  setoid_rewrite Nat2Z.inj_succ. setoid_rewrite <-Z.add_1_l.
-  setoid_rewrite <-loc_add_assoc.
-  rewrite big_opM_singleton; iDestruct "Hvs" as "[$ Hvs]". by iApply "IH".
-Qed.
-
-Lemma wp_allocN_seq s E v n (Φ : expr → iProp Σ) :
-  0 < n →
-  ▷ (∀ (l:loc), ([∗ list] i ∈ seq 0 (Z.to_nat n),
-                 (l +ₗ (i : nat)) ↦ v ∗ meta_token (l +ₗ (i : nat)) ⊤) -∗ Φ #l) -∗
-  sswp s E (AllocN (Val $ LitV $ LitInt $ n) (Val v)) Φ.
-Proof.
-  clear INDEP. 
-  iIntros (HnO) "HΦ".
-  rewrite /sswp. simpl.
-  iIntros (σ) "Hσ".
-  iMod fupd_mask_subseteq as "Hclose"; last iModIntro; first by set_solver.
-  iSplit.
-  { iPureIntro. destruct s; [|done]. apply head_prim_reducible. eauto. }
-  iIntros (e2 σ2 efs Hstep). iIntros "!>!>!>".
-  iMod "Hclose".
-  apply head_reducible_prim_step in Hstep; [|eauto].
-  inv_head_step.
-  iMod (gen_heap_alloc_big _ (heap_array l (replicate (Z.to_nat n) v)) with "Hσ")
-    as "(Hσ & Hl & Hm)".
-  { apply heap_array_map_disjoint.
-    rewrite replicate_length Z2Nat.id ?Hexend; auto with lia. }
-  iFrame.
-  iModIntro.
-  iSplit; [|done].
-  iApply "HΦ".
-  iApply big_sepL_sep. iSplitL "Hl".
-  + by iApply heap_array_to_seq_mapsto.
-  + iApply (heap_array_to_seq_meta with "Hm"). by rewrite replicate_length.
-Qed.
-
-Lemma wp_alloc s E v (Φ : expr → iProp Σ) :
-  ▷ (∀ l, l ↦ v -∗ meta_token l ⊤ -∗ Φ (LitV (LitLoc l))) -∗
-  sswp s E (Alloc v) Φ.
-Proof.
-  iIntros "HΦ". iApply wp_allocN_seq; [lia|].
-  iIntros "!>" (l) "[[Hl Hm] _]". rewrite loc_add_0.
-  iApply ("HΦ" with "Hl Hm").
-Qed.
-
-Lemma wp_choose_nat s E (Φ : expr → iProp Σ) :
-  ▷ (∀ (n:nat), Φ $ Val $ LitV (LitInt n)) -∗
-  sswp s E ChooseNat Φ.
-Proof.
-  clear INDEP. 
-  iIntros "HΦ".
-  rewrite /sswp. simpl.
-  iIntros (σ) "Hσ".
-  iMod fupd_mask_subseteq as "Hclose"; last iModIntro; first by set_solver.
-  iSplit.
-  { iPureIntro. destruct s; [|done]. apply head_prim_reducible. eauto. }
-  iIntros (e2 σ2 efs Hstep). iIntros "!>!>!>".
-  iMod "Hclose".
-  apply head_reducible_prim_step in Hstep; [|eauto].
-  inv_head_step.
-  iFrame.
-  iModIntro.
-  iSplit; [|done].
-  iApply "HΦ".
-  Unshelve. all: apply O.
-Qed.
-
-Lemma wp_load s E l q v (Φ : expr → iProp Σ) :
-  ▷ l ↦{q} v -∗
-  ▷ (l ↦{q} v -∗ Φ v) -∗
-  sswp s E (Load (Val $ LitV $ LitLoc l)) Φ.
-Proof.
-  clear INDEP.
-  iIntros ">Hl HΦ".
-  rewrite /sswp. simpl.
-  iIntros (σ) "Hσ".
-  iMod fupd_mask_subseteq as "Hclose"; last iModIntro; first by set_solver.
-  iDestruct (@gen_heap_valid with "Hσ Hl") as %Hheap.
-  iSplit.
-  { iPureIntro. destruct s; [|done]. apply head_prim_reducible. eauto. }
-  iIntros (e2 σ2 efs Hstep). iIntros "!>!>!>".
-  iMod "Hclose".
-  apply head_reducible_prim_step in Hstep; [|eauto].
-  inv_head_step.
-  iFrame.
-  iModIntro.
-  iSplit; [|done].
-  by iApply "HΦ".
-Qed.
-
-Lemma wp_store s E l v' v (Φ : expr → iProp Σ) :
-  ▷ l ↦ v' -∗
-  ▷ (l ↦ v -∗ Φ $ LitV LitUnit) -∗
-  sswp s E (Store (Val $ LitV (LitLoc l)) (Val v)) Φ.
-Proof.
-  clear INDEP. 
-  iIntros ">Hl HΦ". simpl.
-  iIntros (σ1) "Hsi".
-  iDestruct (gen_heap_valid with "Hsi Hl") as %Hheap.
-  iApply fupd_mask_intro; [set_solver|]. iIntros "Hclose".
-  iSplit.
-  { destruct s; [|done]. iPureIntro. apply head_prim_reducible. by eauto. }
-  iIntros (e2 σ2 efs Hstep). iIntros "!>!>!>".
-  iMod "Hclose".
-  iMod (@gen_heap_update with "Hsi Hl") as "[Hsi Hl]".
-  iFrame.
-  apply head_reducible_prim_step in Hstep; [|by eauto].
-  inv_head_step. iFrame. iModIntro. iSplit; [|done]. by iApply "HΦ".
-Qed.
-
-Lemma wp_cmpxchg_fail s E l q v' v1 v2 (Φ : expr → iProp Σ) :
-  v' ≠ v1 → vals_compare_safe v' v1 →
-  ▷ l ↦{q} v' -∗
-  ▷ (l ↦{q} v' -∗ Φ $ PairV v' (LitV $ LitBool false)) -∗
-  sswp s E (CmpXchg (Val $ LitV $ LitLoc l) (Val v1) (Val v2)) Φ.
-Proof.
-  clear INDEP. 
-  iIntros (??) ">Hl HΦ". simpl.
-  iIntros (σ1) "Hsi".
-  iDestruct (gen_heap_valid with "Hsi Hl") as %Hheap.
-  iApply fupd_mask_intro; [set_solver|]. iIntros "Hclose".
-  iSplit.
-  { destruct s; [|done]. iPureIntro. apply head_prim_reducible. by eauto. }
-  iIntros (e2 σ2 efs Hstep). iIntros "!>!>!>".
-  iMod "Hclose".
-  iFrame.
-  apply head_reducible_prim_step in Hstep; [|by eauto].
-  inv_head_step.
-  rewrite bool_decide_false //. iFrame. iModIntro.
-  iSplit; [|done].
-  by iApply "HΦ".
-Qed.
-
-Lemma wp_cmpxchg_suc s E l v' v1 v2 (Φ : expr → iProp Σ) :
-  v' = v1 → vals_compare_safe v' v1 →
-  ▷ l ↦ v' -∗
-  ▷ (l ↦ v2 -∗ Φ $ PairV v' (LitV $ LitBool true)) -∗
-  sswp s E (CmpXchg (Val $ LitV $ LitLoc l) (Val v1) (Val v2)) Φ.
-Proof.
-  clear INDEP. 
-  iIntros (??) ">Hl HΦ". simpl.
-  iIntros (σ1) "Hsi".
-  iDestruct (gen_heap_valid with "Hsi Hl") as %Hheap.
-  iApply fupd_mask_intro; [set_solver|]. iIntros "Hclose".
-  iSplit.
-  { destruct s; [|done]. iPureIntro. apply head_prim_reducible. by eauto. }
-  iIntros (e2 σ2 efs Hstep). iIntros "!>!>!>".
-  iMod (@gen_heap_update with "Hsi Hl") as "[Hsi Hl]".
-  iMod "Hclose".
-  iFrame.
-  apply head_reducible_prim_step in Hstep; [|by eauto].
-  inv_head_step.
-  rewrite bool_decide_true //. iFrame. iModIntro.
-  iSplit; [|done].
-  by iApply "HΦ".
 Qed.
 
 End lifting.
