fairis/heap_lang/iris_inst.v
@@ -1,0 +1,375 @@
+From iris.proofmode Require Import tactics.
+From iris.base_logic Require Export gen_heap.
+From trillium.program_logic Require Export weakestpre adequacy.
+From trillium.fairness Require Import action_model resources fuel.
+From trillium.fairness.heap_lang Require Export lang tactics notation.
+
+Set Default Proof Using "Type".
+
+
+(* Class heapGpreS Σ `(LM: LiveModel heap_lang M) := HeapPreG { *)
+Class heapGpreS Σ (AM1 AM2: ActionModel) := HeapPreG {
+  heapGpreS_inv :> invGpreS Σ;
+  heapGpreS_gen_heap :> gen_heapGpreS loc val Σ;
+  heapGpreS_fairness :> fairnessGpreS AM1 AM2 Σ;
+}.
+
+(* Class heapGS Σ `(LM:LiveModel heap_lang M) := HeapG { *)
+Class heapGS Σ (AM1 AM2: ActionModel) := HeapG { 
+  heap_inG :> heapGpreS Σ AM1 AM2;
+  heap_invGS : invGS_gen HasNoLc Σ;
+  heap_gen_heapGS :> gen_heapGS loc val Σ;
+  heap_fairnessGS :> fairnessGS AM1 AM2 Σ;
+}.
+
+Definition heapΣ (AM1 AM2: ActionModel) : gFunctors :=
+  #[ invΣ; gen_heapΣ loc val; fairnessΣ heap_lang AM1 AM2 ].
+
+Global Instance subG_heapPreG {Σ} {AM1 AM2: ActionModel} :
+  subG (heapΣ AM1 AM2) Σ → heapGpreS Σ AM1 AM2.
+Proof. solve_inG. Qed.
+
+#[global] Instance heapG_irisG {AM1 AM2: ActionModel} 
+  (PM := ProdAM AM1 AM2)
+  {PMS: AM_strong_lr PM}
+  (M := AM2FM PM PMS)
+  {LM: LiveModel heap_lang M}
+ `{!heapGS Σ AM1 AM2} : irisG heap_lang LM Σ := {
+    iris_invGS := heap_invGS;
+    state_interp extr auxtr :=
+      (⌜valid_state_evolution_fairness extr auxtr⌝ ∗
+       gen_heap_interp (trace_last extr).2.(heap) ∗
+       model_state_interp (trace_last extr).1 (trace_last auxtr))%I ;
+    fork_post tid := λ _, (tid ↦M ∅)%I;
+}.
+
+(** Override the notations so that scopes and coercions work out *)
+Notation "l ↦{ q } v" := (pointsto (L:=loc) (V:=val) l (DfracOwn q) v%V)
+  (at level 20, q at level 50, format "l  ↦{ q }  v") : bi_scope.
+Notation "l ↦ v" :=
+  (pointsto (L:=loc) (V:=val) l (DfracOwn 1) v%V) (at level 20) : bi_scope.
+Notation "l ↦{ q } -" := (∃ v, l ↦{q} v)%I
+  (at level 20, q at level 50, format "l  ↦{ q }  -") : bi_scope.
+Notation "l ↦ -" := (l ↦{1} -)%I (at level 20) : bi_scope.
+
+(** The tactic [inv_head_step] performs inversion on hypotheses of the shape
+[head_step]. The tactic will discharge head-reductions starting from values, and
+simplifies hypothesis related to conversions from and to values, and finite map
+operations. This tactic is slightly ad-hoc and tuned for proving our lifting
+lemmas. *)
+Ltac inv_head_step :=
+  repeat match goal with
+  | _ => progress simplify_map_eq/= (* simplify memory stuff *)
+  | H : to_val _ = Some _ |- _ => apply of_to_val in H
+  | H : head_step ?e _ _ _ _ |- _ =>
+     try (is_var e; fail 1); (* inversion yields many goals if [e] is a variable
+     and can thus better be avoided. *)
+     inversion H; subst; clear H
+  end.
+
+Hint Extern 0 (head_reducible _ _) => eexists _, _, _; simpl : core.
+Hint Extern 1 (head_step _ _ _ _ _) => econstructor : core.
+Hint Extern 0 (head_step (CmpXchg _ _ _) _ _ _ _) => eapply CmpXchgS : core.
+Hint Extern 0 (head_step (AllocN _ _) _ _ _ _) => apply alloc_fresh : core.
+Hint Resolve to_of_val : core.
+
+#[global] Instance into_val_val v : IntoVal (Val v) v.
+Proof. done. Qed.
+#[global] Instance as_val_val v : AsVal (Val v).
+Proof. by eexists. Qed.
+
+Local Ltac solve_atomic :=
+  apply strongly_atomic_atomic, ectx_language_atomic;
+    [inversion 1; naive_solver
+    |apply ectxi_language_sub_redexes_are_values; intros [] **; naive_solver].
+
+#[global] Instance rec_atomic s f x e : Atomic s (Rec f x e).
+Proof. solve_atomic. Qed.
+#[global] Instance pair_atomic s v1 v2 : Atomic s (Pair (Val v1) (Val v2)).
+Proof. solve_atomic. Qed.
+#[global] Instance injl_atomic s v : Atomic s (InjL (Val v)).
+Proof. solve_atomic. Qed.
+#[global] Instance injr_atomic s v : Atomic s (InjR (Val v)).
+Proof. solve_atomic. Qed.
+(** The instance below is a more general version of [Skip] *)
+#[global] Instance beta_atomic s f x v1 v2 : Atomic s (App (RecV f x (Val v1)) (Val v2)).
+Proof. destruct f, x; solve_atomic. Qed.
+#[global] Instance unop_atomic s op v : Atomic s (UnOp op (Val v)).
+Proof. solve_atomic. Qed.
+#[global] Instance binop_atomic s op v1 v2 : Atomic s (BinOp op (Val v1) (Val v2)).
+Proof. solve_atomic. Qed.
+#[global] Instance if_true_atomic s v1 e2 : Atomic s (If (Val $ LitV $ LitBool true) (Val v1) e2).
+Proof. solve_atomic. Qed.
+#[global] Instance if_false_atomic s e1 v2 : Atomic s (If (Val $ LitV $ LitBool false) e1 (Val v2)).
+Proof. solve_atomic. Qed.
+#[global] Instance fst_atomic s v : Atomic s (Fst (Val v)).
+Proof. solve_atomic. Qed.
+#[global] Instance snd_atomic s v : Atomic s (Snd (Val v)).
+Proof. solve_atomic. Qed.
+
+#[global] Instance fork_atomic s e : Atomic s (Fork e).
+Proof. solve_atomic. Qed.
+
+#[global] Instance allocN_atomic s v w : Atomic s (AllocN (Val v) (Val w)).
+Proof. solve_atomic. Qed.
+#[global] Instance alloc_atomic s v : Atomic s (Alloc (Val v)).
+Proof. solve_atomic. Qed.
+#[global] Instance load_atomic s v : Atomic s (Load (Val v)).
+Proof. solve_atomic. Qed.
+#[global] Instance store_atomic s v1 v2 : Atomic s (Store (Val v1) (Val v2)).
+Proof. solve_atomic. Qed.
+#[global] Instance cmpxchg_atomic s v0 v1 v2 : Atomic s (CmpXchg (Val v0) (Val v1) (Val v2)).
+Proof. solve_atomic. Qed.
+#[global] Instance faa_atomic s v1 v2 : Atomic s (FAA (Val v1) (Val v2)).
+Proof. solve_atomic. Qed.
+
+Local Ltac solve_exec_safe := intros; subst; do 3 eexists; econstructor; eauto.
+Local Ltac solve_exec_puredet := simpl; intros; by inv_head_step.
+Local Ltac solve_pure_exec :=
+  subst; intros ?; apply nsteps_once, pure_head_step_pure_step;
+    constructor; [solve_exec_safe | solve_exec_puredet].
+
+(** The behavior of the various [wp_] tactics with regard to lambda differs in
+the following way:
+
+- [wp_pures] does *not* reduce lambdas/recs that are hidden behind a definition.
+- [wp_rec] and [wp_lam] reduce lambdas/recs that are hidden behind a definition.
+
+To realize this behavior, we define the class [AsRecV v f x erec], which takes a
+value [v] as its input, and turns it into a [RecV f x erec] via the instance
+[AsRecV_recv : AsRecV (RecV f x e) f x e]. We register this instance via
+[Hint Extern] so that it is only used if [v] is syntactically a lambda/rec, and
+not if [v] contains a lambda/rec that is hidden behind a definition.
+
+To make sure that [wp_rec] and [wp_lam] do reduce lambdas/recs that are hidden
+behind a definition, we activate [AsRecV_recv] by hand in these tactics. *)
+Class AsRecV (v : val) (f x : binder) (erec : expr) :=
+  as_recv : v = RecV f x erec.
+#[global] Hint Mode AsRecV ! - - - : typeclass_instances.
+Definition AsRecV_recv f x e : AsRecV (RecV f x e) f x e := eq_refl.
+#[global] Hint Extern 0 (AsRecV (RecV _ _ _) _ _ _) =>
+  apply AsRecV_recv : typeclass_instances.
+
+#[global] Instance pure_recc f x (erec : expr) :
+  PureExec True 1 (Rec f x erec) (Val $ RecV f x erec).
+Proof. solve_pure_exec. Qed.
+#[global] Instance pure_pairc (v1 v2 : val) :
+  PureExec True 1 (Pair (Val v1) (Val v2)) (Val $ PairV v1 v2).
+Proof. solve_pure_exec. Qed.
+#[global] Instance pure_injlc (v : val) :
+  PureExec True 1 (InjL $ Val v) (Val $ InjLV v).
+Proof. solve_pure_exec. Qed.
+#[global] Instance pure_injrc (v : val) :
+  PureExec True 1 (InjR $ Val v) (Val $ InjRV v).
+Proof. solve_pure_exec. Qed.
+
+#[global] Instance pure_beta f x (erec : expr) (v1 v2 : val) `{!AsRecV v1 f x erec} :
+  PureExec True 1 (App (Val v1) (Val v2)) (subst' x v2 (subst' f v1 erec)).
+Proof. unfold AsRecV in *. solve_pure_exec. Qed.
+
+#[global] Instance pure_unop op v v' :
+  PureExec (un_op_eval op v = Some v') 1 (UnOp op (Val v)) (Val v').
+Proof. solve_pure_exec. Qed.
+
+#[global] Instance pure_binop op v1 v2 v' :
+  PureExec (bin_op_eval op v1 v2 = Some v') 1 (BinOp op (Val v1) (Val v2)) (Val v') | 10.
+Proof. solve_pure_exec. Qed.
+(* Higher-priority instance for [EqOp]. *)
+#[global] Instance pure_eqop v1 v2 :
+  PureExec (vals_compare_safe v1 v2) 1
+    (BinOp EqOp (Val v1) (Val v2))
+    (Val $ LitV $ LitBool $ bool_decide (v1 = v2)) | 1.
+Proof.
+  intros Hcompare.
+  cut (bin_op_eval EqOp v1 v2 = Some $ LitV $ LitBool $ bool_decide (v1 = v2)).
+  { intros. revert Hcompare. solve_pure_exec. }
+  rewrite /bin_op_eval /= decide_True //.
+Qed.
+
+#[global] Instance pure_if_true e1 e2 : PureExec True 1 (If (Val $ LitV $ LitBool true) e1 e2) e1.
+Proof. solve_pure_exec. Qed.
+
+#[global] Instance pure_if_false e1 e2 : PureExec True 1 (If (Val $ LitV  $ LitBool false) e1 e2) e2.
+Proof. solve_pure_exec. Qed.
+
+#[global] Instance pure_fst v1 v2 :
+  PureExec True 1 (Fst (Val $ PairV v1 v2)) (Val v1).
+Proof. solve_pure_exec. Qed.
+
+#[global] Instance pure_snd v1 v2 :
+  PureExec True 1 (Snd (Val $ PairV v1 v2)) (Val v2).
+Proof. solve_pure_exec. Qed.
+
+#[global] Instance pure_case_inl v e1 e2 :
+  PureExec True 1 (Case (Val $ InjLV v) e1 e2) (App e1 (Val v)).
+Proof. solve_pure_exec. Qed.
+
+#[global] Instance pure_case_inr v e1 e2 :
+  PureExec True 1 (Case (Val $ InjRV v) e1 e2) (App e2 (Val v)).
+Proof. solve_pure_exec. Qed.
+
+
+(* TODO: move to corresponding files? *)
+Section SSWP_MU.
+
+  Context {AM1 AM2: ActionModel}.
+  Let PM := ProdAM AM1 AM2.
+  Context {PROD_LR: AM_strong_lr PM}.
+  Let M := AM2FM PM PROD_LR.
+  Context {LM: LiveModel heap_lang M}.
+  Context `{hGS: !heapGS Σ AM1 AM2}.
+  
+  (* Need to explicitly specify the instance, 
+     since the LM argument is not inferred automatically *)
+  Let hi := @heapG_irisG AM1 AM2 PROD_LR LM _ hGS. 
+  Existing Instance hi. 
+
+  Definition sswp (s : stuckness) E e1 (Φ : expr → iProp Σ) : iProp Σ :=
+    match to_val e1 with
+    | Some v => |={E}=> (Φ (of_val v))
+    | None => ∀ σ1,
+        gen_heap_interp σ1.(heap) ={E,∅}=∗
+        ⌜if s is NotStuck then reducible e1 σ1 else True⌝ ∗
+        ∀ e2 σ2 efs, ⌜prim_step e1 σ1 e2 σ2 efs⌝ ={∅}▷=∗ |={∅,E}=>
+        gen_heap_interp σ2.(heap) ∗ Φ e2 ∗ ⌜efs = []⌝
+    end%I.
+
+  Lemma sswp_wand s e E (Φ Ψ : expr → iProp Σ) :
+    (∀ e, Φ e -∗ Ψ e) -∗ sswp s E e Φ -∗ sswp s E e Ψ.
+  Proof.
+    rewrite /sswp. iIntros "HΦΨ HΦ".
+    destruct (to_val e); [by iApply "HΦΨ"|].
+    iIntros (?) "H". iMod ("HΦ" with "H") as "[%Hs HΦ]".
+    iModIntro. iSplit; [done|]. iIntros (????).
+    iDestruct ("HΦ" with "[//]") as "HΦ".
+    iMod "HΦ". iIntros "!>!>". iMod "HΦ". iIntros "!>". iMod "HΦ" as "(?&?&?)".
+    iIntros "!>". iFrame. by iApply "HΦΨ".
+  Qed.
+
+  Definition HL_LM_trace_interp' (extr: execution_trace heap_lang)
+    (lmtr: auxiliary_trace LM) (τ: locale heap_lang): iProp Σ :=
+    match extr with
+    | {tr[ _ ]} => False
+    | extr' :tr[oζ]: c' =>
+        let c := trace_last extr' in
+        let δ := trace_last lmtr in
+        gen_heap_interp c'.2.(heap) ∗
+        model_state_interp c.1 δ ∗
+        ⌜ tids_smaller c.1 δ ⌝ ∗
+        ⌜ oζ = Some τ ⌝ ∗
+        ⌜ locale_step c (Some τ) c' ⌝
+    end.
+
+    Definition MU E ζ (P : iProp Σ) : iProp Σ :=
+    ∀ extr atr,
+      HL_LM_trace_interp' extr atr ζ ={E}=∗
+      ∃ δ2 ℓ, state_interp extr (trace_extend atr ℓ δ2) ∗ P.
+
+  Lemma MU_wand E ζ (P Q : iProp Σ) :
+    (P -∗ Q) -∗ MU E ζ P -∗ MU E ζ Q.
+  Proof.
+    rewrite /MU. iIntros "HPQ HMU".
+    iIntros (extr atr) "Hσ".
+    iMod ("HMU" with "Hσ") as (??) "[Hσ HP]". iModIntro.
+    iExists _, _. iFrame. by iApply "HPQ".
+  Qed.
+
+  Lemma MU_mask_weaken E1 E2 ζ (P: iProp Σ)
+    (SUB: E1 ⊆ E2):
+    MU E1 ζ P -∗ MU E2 ζ P.
+  Proof.
+    rewrite /MU. iIntros "MU".
+    iIntros "**".
+    iApply fupd_mask_mono; eauto.
+    by iApply "MU". 
+  Qed.
+
+  (* TODO: unify with existing locales_of_list_from_locale_from, 
+     remove restriction for Λ *)
+  Lemma locales_of_list_from_locale_from' {Λ: language} `{EqDecision (locale Λ)}
+    tp0 tp1 ζ:
+    ζ ∈ locales_of_list_from tp0 tp1 (Λ := Λ) ->
+    is_Some (from_locale_from tp0 tp1 ζ).
+  Proof.
+    clear -tp0 tp1 ζ.
+    revert tp0; induction tp1 as [|e1 tp1 IH]; intros tp0.
+    { simpl. intros H. inversion H. }
+    simpl.
+    rewrite /locales_of_list_from /=. intros.
+    destruct (decide (language.locale_of tp0 e1 = ζ)); simplify_eq; first set_solver.
+    apply elem_of_cons in H as [?| ?]; [done| ].
+    set_solver.
+  Qed.
+
+  (* TODO: have similar proof in other repo *)
+  Lemma MSI_tids_smaller (σ: list expr) δ:
+    ⊢ model_state_interp σ δ -∗ ⌜tids_smaller σ δ⌝.
+  Proof. 
+    rewrite /model_state_interp.
+    iIntros "(%fm & %LE & %DEAD & %TP & X)".
+    iPureIntro. red. intros.
+    apply locales_of_list_from_locale_from'.
+    destruct (decide (ζ ∈ locales_of_list σ)); [done| ].
+    red in TP. specialize (TP _ n).
+    red in LE. apply proj2 in LE. rewrite -LE in H.
+    by apply not_elem_of_dom in TP. 
+  Qed. 
+  
+  Lemma sswp_MU_wp_fupd s E E' ζ e Φ
+    (NVAL: language.to_val e = None)
+    :
+    let sswp_post := λ e', (MU E' ζ ((|={E',E}=> WP e' @ s; ζ; E {{ Φ }})))%I in
+      (|={E,E'}=> sswp s E' e sswp_post)%I -∗
+      WP e @ s; ζ; E {{ Φ }}.
+  Proof.
+    simpl. rewrite wp_unfold /wp_pre.
+    iIntros "Hsswp". rewrite NVAL. 
+    iIntros (extr atr K tp1 tp2 σ1 Hvalid Hζ Hextr) "Hσ".
+    iMod "Hsswp" as "foo".
+    rewrite /sswp. rewrite NVAL.
+    iSimpl in "Hσ". iDestruct "Hσ" as "(%EV & HEAP & MSI)".
+    iSpecialize ("foo" with "HEAP").
+    iMod "foo" as (Hs) "Hsswp".
+    red in Hextr. rewrite Hextr. 
+    iModIntro. iSplit.
+    { iPureIntro. by rewrite Hextr in Hs. }
+    iIntros (e2 σ2 efs Hstep).
+    iDestruct ("Hsswp" with "[//]") as "Hsswp".
+    iApply (step_fupdN_le 1); [| done| ].
+    { pose proof (trace_length_at_least extr). lia. }
+    simpl.
+    iApply (step_fupd_wand with "Hsswp").
+    iIntros ">(Hσ & HMU & ->)".
+    rewrite /MU. iSpecialize ("HMU" $! (_ :tr[Some ζ]: _)  with "[MSI Hσ]").
+    { rewrite /HL_LM_trace_interp'.
+      iPoseProof (MSI_tids_smaller with "MSI") as "%TS".
+      remember (trace_last extr) as xx. destruct xx as [tp h].
+      inversion Hextr as [[TP H]]. 
+      rewrite -TP in TS. 
+      iApply bi.sep_assoc. iSplitL.
+      2: { iPureIntro. repeat split; eauto.
+           { replace tp with (tp, h).1 in TS by done.
+             rewrite Heqxx in TS. apply TS. }
+           simpl in Hζ. 
+           rewrite -Hζ. simpl.
+           (* rewrite locale_fill'.  *)
+           eapply locale_step_atomic.
+           3: { eapply @fill_step. apply Hstep. } 
+           { rewrite -Heqxx Hextr. simpl. reflexivity. }
+           reflexivity. }
+      rewrite -Heqxx TP. simpl. iFrame. }
+    iMod ("HMU") as (??) "[Hσ Hwp]". iMod "Hwp". iModIntro.
+    iExists _, _. rewrite right_id_L. by iFrame.
+  Qed.
+
+  Lemma sswp_MU_wp s E ζ e (Φ : val → iProp Σ)
+    (NVAL: language.to_val e = None):
+    sswp s E e (λ e', MU E ζ (WP e' @ s; ζ;  E {{ Φ }})) -∗
+      WP e @ s; ζ; E {{ Φ }}.
+  Proof.
+    iIntros "Hsswp". iApply sswp_MU_wp_fupd; auto. iModIntro.
+    iApply (sswp_wand with "[] Hsswp").
+    iIntros (?) "HMU". iApply (MU_wand with "[] HMU"). by iIntros "$ !>".
+  Qed.
+
+End SSWP_MU.
